BinNat

Auto/Lib/BinNat.lean
@@ -1,3 +1,5 @@
+import Std.Data.Nat.Lemmas
+
 inductive Pos where
   | xH : Pos
   | xO : Pos → Pos
@@ -11,6 +13,188 @@ inductive Bin where
   | pos : Pos → Bin
 
 abbrev Bin.one := pos .xH
+
+def Pos.toNat : Pos → Nat
+| xH => 1
+| xO p' => p'.toNat * 2
+| xI p' => p'.toNat * 2 + 1
+
+theorem Pos.toNat_not_zero (p : Pos) : Pos.toNat p ≠ 0 := by
+  induction p
+  case xH => intro H; contradiction
+  case xO p' IH =>
+    simp [Pos.toNat]; intro H
+    rw [Nat.mul_eq_zero] at H
+    cases H
+    case inl H' => revert H'; exact IH
+    case inr H' => cases H'
+  case xI p' _ =>
+    simp [Pos.toNat] 
+
+theorem Pos.ofNatWF_rec_lemma (n : Nat) : n ≥ 2 → n / 2 < n := by
+  intro H; apply Nat.div_lt_self
+  case hLtN =>
+    cases n;
+    contradiction;
+    apply Nat.succ_le_succ; apply Nat.zero_le
+  case hLtK => apply Nat.le_refl
+
+theorem Pos.ofNatWF_rec_lemma' (n n' : Nat) : n = n' + 2 → n / 2 < n := by
+  intro h; apply ofNatWF_rec_lemma; rw [h];
+  apply Nat.succ_le_succ; apply Nat.succ_le_succ;
+  apply Nat.zero_le
+
+def Pos.ofNatWF (n : Nat) :=
+  match h : n with
+  | 0 => xH
+  | 1 => xH
+  | _ + 2 =>
+    match n % 2 with
+    | 0 => .xO (Pos.ofNatWF (n / 2))
+    | _ => .xI (Pos.ofNatWF (n / 2))
+decreasing_by apply Pos.ofNatWF_rec_lemma'; assumption
+
+theorem Pos.ofNatWF.inductionOn.{u}
+  {motive : Nat → Sort u} (x : Nat)
+  (ind : ∀ x, motive ((x + 2) / 2) → motive (x + 2))
+  (base₀ : motive 0) (base₁ : motive 1) : motive x :=
+  match h : x with
+  | 0 => base₀
+  | 1 => base₁
+  | x' + 2 => ind x' (inductionOn ((x' + 2) / 2) ind base₀ base₁)
+decreasing_by apply Pos.ofNatWF_rec_lemma'; rfl
+
+theorem Pos.ofNatWF.induction
+  {motive : Nat → Sort u}
+  (ind : ∀ x, motive ((x + 2) / 2) → motive (x + 2))
+  (base₀ : motive 0) (base₁ : motive 1) : ∀ x, motive x :=
+  fun x => Pos.ofNatWF.inductionOn x ind base₀ base₁
+
+theorem Pos.ofNatWF.succSucc (n : Nat) :
+  Pos.ofNatWF (n + 2) =
+    match (n + 2) % 2 with
+    | 0 => .xO (Pos.ofNatWF ((n + 2) / 2))
+    | _ => .xI (Pos.ofNatWF ((n + 2) / 2)) := rfl
+
+theorem Pos.ofNatWF.double_xO (n : Nat) :
+  n ≠ 0 → Pos.ofNatWF (n * 2) = xO (Pos.ofNatWF n) :=
+  match n with
+  | 0 => by intro H; contradiction
+  | 1 => fun _ => by simp [ofNatWF]
+  | n' + 2 => fun H => by
+    simp; rw [Nat.mul_comm, Nat.mul_add];
+    rw [Pos.ofNatWF.succSucc];
+    have heq : (2 * n' + 2 + 2) % 2 = 0 := by
+      rw [Nat.add_mod_right]; rw [Nat.add_mod_right]
+      rw [Nat.mul_mod]; simp
+    rw [heq]; simp
+
+theorem Pos.ofNatWF.doubleSucc_xI (n : Nat) :
+  n ≠ 0 → Pos.ofNatWF ((n * 2) + 1) = xI (Pos.ofNatWF n) :=
+  match n with
+  | 0 => by intro H; contradiction
+  | 1 => fun _ => by simp [ofNatWF]
+  | n' + 2 => fun H => by
+    simp; rw [Nat.mul_comm, Nat.mul_add];
+    have : (2 * n' + 2 * 2 + 1) = (2 * n') + 3 + 2 := rfl
+    rw [Pos.ofNatWF.succSucc];
+    have heq : (2 * n' + 3 + 2) % 2 = 1 := by
+      rw [Nat.add_mod_right]; rw [Nat.add_mod]
+      rw [Nat.mul_mod]; simp
+    rw [heq]; simp
+    have heq' : Nat.succ ((2 * n' + 3) / 2) = n' + 2 := by
+      apply congrArg; rw [Nat.add_comm];
+      rw [Nat.add_mul_div_left _ _ (by simp)]; rw [Nat.add_comm]; rfl;
+    rw [heq']
+
+theorem Pos.ofNatWF_toNat (p : Pos) : Pos.ofNatWF (Pos.toNat p) = p := by
+  induction p
+  case xH => rfl
+  case xO p' IH =>
+    dsimp [Pos.toNat];
+    rw [Pos.ofNatWF.double_xO];
+    rw [IH]; apply Pos.toNat_not_zero
+  case xI p' IH =>
+    dsimp [Pos.toNat];
+    rw [Pos.ofNatWF.doubleSucc_xI];
+    rw [IH]; apply Pos.toNat_not_zero
+
+theorem Pos.toNat_ofNatWF (n : Nat) : n ≠ 0 → Pos.toNat (Pos.ofNatWF n) = n := by
+  revert n; apply Pos.ofNatWF.induction
+  case base₀ => intro H; contradiction
+  case base₁ => intro H; rfl
+  case ind =>
+    intro x IH _
+    have hne : (x + 2) / 2 ≠ 0 := by
+      rw [Nat.add_div_right]; simp; simp
+    have IH' := IH hne
+    rw [ofNatWF.succSucc];
+    have heq : (x + 2) / 2 = Nat.succ (x / 2) := Nat.add_div_right _ (by simp)
+    rw [heq] at IH'
+    match h : (x + 2) % 2 with
+    | 0 =>
+      simp [toNat]; rw [IH'];
+      rw [← Nat.mod_add_div (x + 2) 2];
+      rw [h]; simp; apply Nat.mul_comm
+    | 1 =>
+      simp [toNat]; rw [IH'];
+      rw [Nat.add_mul _ 1]; simp
+      calc
+        _ = 2 * (x / 2) + x % 2 := by
+          rw [Nat.add_mod_right] at h
+          rw [h]; rw [Nat.mul_comm]
+        _ = _ := by apply Nat.div_add_mod
+    | w' + 2 =>
+      have h' := Nat.not_lt_of_le (Nat.le_of_eq (Eq.symm h))
+      apply False.elim; apply h'
+      apply Nat.le_trans (m:=2)
+      apply Nat.mod_lt; simp
+      apply Nat.succ_le_succ; apply Nat.succ_le_succ; apply Nat.zero_le
+
+def Pos.ofNatRD (rd : Nat) (n : Nat) :=
+  match rd with
+  | 0 => xH
+  | .succ rd' =>
+    match n with
+    | 0 => xH
+    | 1 => xH
+    | _ =>
+      match Nat.mod n 2 with
+      | 0 => .xO (Pos.ofNatRD rd' (Nat.div n 2))
+      | _ => .xI (Pos.ofNatRD rd' (Nat.div n 2))
+
+theorem Pos.ofNat.equivAux (rd n : Nat) : rd ≥ n → Pos.ofNatWF n = Pos.ofNatRD rd n := by
+  revert n; induction rd <;> intros n H
+  case zero =>
+    have hzero : n = 0 := Nat.eq_zero_of_le_zero H
+    rw [hzero]; rfl
+  case succ rd' IH =>
+    dsimp [ofNatRD]
+    match n with
+    | 0 => rfl
+    | 1 => rfl
+    | n' + 2 =>
+      rw [Pos.ofNatWF.succSucc]; simp;
+      have heq' : Nat.mod (n' + 2) 2 = n' % 2 := by
+        suffices (n' + 2) % 2 = n' % 2 by exact this
+        rw [Nat.add_mod_right]
+      have heqDiv : Nat.div (n' + 2) 2 = Nat.succ (n' / 2) := by
+        suffices (n' + 2) / 2 = Nat.succ (n' / 2) by exact this
+        rw [Nat.add_div_right]; simp
+      rw [IH, heq', heqDiv];
+      apply Nat.le_trans (m := n' + 1)
+      case a.a => apply Nat.succ_le_succ; apply Nat.div_le_self
+      case a.a => apply Nat.le_of_succ_le_succ H
+
+def Pos.ofNat n := Pos.ofNatRD n n
+
+theorem Pos.ofNat.equiv (n : Nat) : Pos.ofNatWF n = Pos.ofNat n :=
+  Pos.ofNat.equivAux n n (Nat.le_refl _)
+
+def Bin.ofNat (n : Nat) : Bin :=
+  match n with
+  | 0 => zero
+  | _ => pos (Pos.ofNat n)
 
 def Pos.beq : (p q : Pos) → Bool
 | xH,    xH    => true
@@ -37,15 +221,6 @@ theorem Pos.beq_eq : (p q : Pos) → p.beq q = true → p = q
 
 instance : BEq Pos where
   beq := Pos.beq
-
-private partial def Pos.ofNatAux (n : Nat) :=
-  match n with
-  | 0 => xH
-  | 1 => xH
-  | _ =>
-    match n % 2 with
-    | 0 => .xO (Pos.ofNatAux (n / 2))
-    | _ => .xI (Pos.ofNatAux (n / 2))
 
 def Pos.succ (p : Pos) : Pos :=
   match p with
@@ -116,4 +291,3 @@ theorem Pos.neq_XH_succ_pred_eq (p : Pos) : p ≠ .xH → Pos.succ (Pos.pred p) 
 
 theorem Pos.succ_inj (p q : Pos) : Pos.succ p = Pos.succ q → p = q := fun H =>
   Pos.pred_succ_eq p ▸ Pos.pred_succ_eq q ▸ (congrArg _ H : pred (succ p) = pred (succ q))
-
